First fully closed proof of an optimization: moving reads down w/ protectors

theories/tree_borrows/examples/lib.v
@@ -3,29 +3,42 @@ From simuliris.tree_borrows Require Import primitive_laws proofmode steps_progre
 From iris.prelude Require Import options.
 
 
-(* Allocate a place of type [T] and initialize it with a value [v] *)
-Definition new_place T (v: expr) : expr :=
-  let: "x" := Alloc T in "x" <- v ;; "x".
+(* Allocate a place of size [sz] and initialize it with a value [v] *)
+Definition new_place sz (v: expr) : expr :=
+  let: "x" := Alloc sz in "x" <- v ;; "x".
 
-(* Retag a place [p] that is a pointer of kind [pk] to a region of type [T],
+(* Retag a place [p] that is a pointer of kind [pk] to a region of size [sz],
   with retag [kind] and call_id [c] *)
 Definition retag_place
-  (p: expr) (pk: pointer_kind) (T: type) (kind: retag_kind) (c : expr) : expr :=
+  (p: expr) (pk: pointer_kind) (sz : nat) (kind: retag_kind) (c : expr) : expr :=
   let: "p" := p in
   (* read the current pointer stored in the place [p] *)
   (* retag and update [p] with the pointer with new tag *)
-  "p" <- Retag (Copy "p") c pk T kind.
+  "p" <- Retag (Copy "p") c pk sz kind.
 
-Lemma sim_new_place_local `{sborGS Σ} T v_t v_s π Φ :
+Lemma write_entire_range {T} l sz (v v' : list T) :
+  length v = sz →
+  length v' = sz →
+  write_range l l v' v = Some v'.
+Proof.
+  intros <- Hlen.
+  rewrite /write_range bool_decide_true. 2: lia. f_equal.
+  eapply list_eq.
+  intros i. eapply write_range_to_list_lookup. split.
+  1: rewrite Z.sub_diag Z2Nat.inj_0 Nat.sub_0_r //.
+  intros H. rewrite !lookup_ge_None_2; try done. all: lia.
+Qed.
+
+Lemma sim_new_place_local `{sborGS Σ} sz v_t v_s π Φ :
   ⌜length v_t = length v_s⌝ -∗
   (∀ t l,
-    ⌜length v_s = tsize T⌝ -∗
-    ⌜length v_t = tsize T⌝ -∗
+    ⌜length v_s = sz⌝ -∗
+    ⌜length v_t = sz⌝ -∗
     t $$ tk_local -∗
     l ↦t∗[tk_local]{t} v_t -∗
     l ↦s∗[tk_local]{t} v_s -∗
-    PlaceR l (Tagged t) T ⪯{π} PlaceR l (Tagged t) T [{ Φ }]) -∗
-  new_place T #v_t ⪯{π} new_place T #v_s [{ Φ }].
+    PlaceR l t sz ⪯{π} PlaceR l t sz [{ Φ }]) -∗
+  new_place sz #v_t ⪯{π} new_place sz #v_s [{ Φ }].
 Proof.
   iIntros (Hlen_eq) "Hsim".
   rewrite /new_place. sim_bind (Alloc _) (Alloc _).
@@ -34,24 +47,29 @@ Proof.
   source_bind (Write _ _).
   (* gain knowledge about the length *)
   iApply source_red_safe_implies. iIntros (Hsize).
-  iApply (source_write_local with "Htag Hs"); [by rewrite replicate_length | done | ].
+  iApply (source_write_local with "Htag Hs"). 2: done.
+  { eapply write_entire_range. 2: exact Hsize. rewrite replicate_length //. }
   iIntros "Hs Htag". source_finish.
 
   target_bind (Write _ _).
-  iApply (target_write_local with "Htag Ht"); [ by rewrite replicate_length | lia| ].
+  iApply (target_write_local with "Htag Ht"). 2: done. 2: lia.
+  { eapply write_entire_range. 1: rewrite replicate_length //. lia. }
   iIntros "Ht Htag". target_finish.
 
   sim_pures. iApply ("Hsim" with "[//] [] Htag Ht Hs").
   iPureIntro; lia.
 Qed.
 
-Lemma new_place_safe_reach P σ T r :
-  safe_reach P (new_place T (of_result r)) σ (λ _ _, ∃ v, r = ValR v ∧ length v = tsize T).
+
+Lemma new_place_safe_reach P σ sz r :
+  safe_reach P (new_place sz (of_result r)) σ (λ _ _, ∃ v, r = ValR v ∧ length v = sz).
 Proof.
   rewrite /new_place.
   safe_reach_bind (Alloc _).
+  eapply safe_reach_safe_implies; first eapply safe_implies_alloc_strong.
+  intros (HH1&HH2).
   eapply safe_reach_base_step.
-  { eapply alloc_base_step. }
+  { econstructor 2. 1: econstructor. econstructor. all: done. }
   eapply safe_reach_refl.
   safe_reach_bind (Let _ _ _).
   eapply safe_reach_pure; [ apply _ | done | ].
@@ -59,8 +77,8 @@ Proof.
   destruct r as [ v | ]; simpl.
   - (* value *)
     safe_reach_bind (Write _ _).
-    eapply safe_reach_safe_implies; [ apply _ | ].
-    intros (_ & _ & ?).
+    eapply safe_reach_safe_implies; [ apply safe_implies_write_weak | ].
+    intros ?.
     do 2 eapply safe_reach_refl. eauto.
   - safe_reach_bind (Write _ _).
     eapply safe_reach_safe_implies; [ apply _ | done].
