theories/tree_borrows/adequacy.v
@@ -10,7 +10,7 @@ Lemma sc_rel_obs `{!sborGS Σ} sc_t sc_s :
   sc_rel sc_t sc_s ⊢@{iPropI Σ} ⌜ obs_scalar sc_t sc_s ⌝.
 Proof.
   destruct sc_t, sc_s; try by eauto.
-  rewrite sc_rel_cid_source. iIntros "[<- _]". eauto.
+  iIntros "(->&_)". done.
 Qed.
 
 Lemma rrel_obs `{!sborGS Σ} r_t r_s :
