theories/tree_borrows/examples/opt1_down.v
@@ -9,19 +9,22 @@ From iris.prelude Require Import options.
 
 (** Moving a read of a mutable reference down across code that *may* use that ref. *)
 
+(* in our simplified memory model, pointers and integers occupy one memory slot *)
+Definition sizeof_scalar : nat := 1.
+
 (* Assuming x : &mut i32 *)
 Definition ex1_down_unopt : expr :=
     let: "c" := InitCall in
     (* "x" is the local variable that stores the pointer value "i" *)
-    let: "x" := new_place (&mut int) "i" in
+    let: "x" := new_place sizeof_scalar "i" in
 
     (* retag_place reborrows the pointer value stored in "x" (which is "i"),
       then updates "x" with the new pointer value. This relies on protectors,
       hence [FnEntry]. *)
-    retag_place "x" (RefPtr Mutable) int FnEntry "c";;
+    retag_place "x" (MutRef TyFrz) sizeof_scalar FnEntry "c";;
 
     (* Read the value "v" from the cell pointed to by the pointer in "x" *)
-    let: "v" := Copy *{int} "x" in
+    let: "v" := Copy *{sizeof_scalar} "x" in
 
     (* The unknown code is represented by a call to an unknown function "f" *)
     Call #[ScFnPtr "f"] #[] ;;
@@ -36,10 +39,10 @@ Definition ex1_down_unopt : expr :=
 
 Definition ex1_down_opt : expr :=
     let: "c" := InitCall in
-    let: "x" := new_place (&mut int) "i" in
-    retag_place "x" (RefPtr Mutable) int FnEntry "c";;
+    let: "x" := new_place sizeof_scalar "i" in
+    retag_place "x" (MutRef TyFrz) sizeof_scalar FnEntry "c";;
     Call #[ScFnPtr "f"] #[] ;;
-    let: "v" := Copy *{int} "x" in
+    let: "v" := Copy *{sizeof_scalar} "x" in
     (* crucial point: need to know that we retain the permission to read *)
 
     Free "x" ;;
@@ -60,62 +63,61 @@ Proof.
   simpl. source_bind (new_place _ _).
   iApply source_red_safe_reach.
   { intros. rewrite subst_result. eapply new_place_safe_reach. }
-  simpl. iIntros "(%v_s & -> & %Hsize)".
+  simpl. iIntros "(%v_s & -> & %Hsize)". destruct v_s as [|v_s [|?]]; try done.
   iPoseProof (rrel_value_source with "Hrel") as (v_t) "(-> & #Hv)".
-  iPoseProof (value_rel_length with "Hv") as "%Hlen".
+  iPoseProof (value_rel_length with "Hv") as "%Hlen". destruct v_t as [|v_t [|?]]; try done.
   iApply source_red_base. iModIntro. to_sim.
   sim_apply (new_place _ _) (new_place _ _) sim_new_place_local "%t %l % % Htag Ht Hs"; first done.
   sim_pures.
 
-  target_apply (Copy _) (target_copy_local with "Htag Ht") "Ht Htag"; first lia.
-  source_apply (Copy _) (source_copy_local with "Htag Hs") "Hs Htag"; first lia.
+  target_apply (Copy _) (target_copy_local with "Htag Ht") "Ht Htag". 2: done. 1: rewrite read_range_heaplet_to_list // Z.sub_diag /= //.
+  source_apply (Copy _) (source_copy_local with "Htag Hs") "Hs Htag". 2: done. 1: rewrite read_range_heaplet_to_list // Z.sub_diag /= //.
 
   (* do the retag *)
   sim_bind (Retag _ _ _ _ _) (Retag _ _ _ _ _).
   iApply sim_safe_implies.
-  iIntros ((_ & ot & i & -> & _)).
-  iPoseProof (value_rel_singleton_source with "Hv") as (sc_t) "[-> Hscrel]".
-  iPoseProof (sc_rel_ptr_source with "Hscrel") as "[-> Htagged]".
-  iApply (sim_retag_fnentry with "Hscrel Hcall"); [cbn; lia| done | ].
-  iIntros (t_i v_t v_s Hlen_t Hlen_s) "#Hvrel Hcall Htag_i Hi_t Hi_s _".
+  iIntros ((_ & ot & i & [= ->] & _)).
+  iPoseProof (value_rel_singleton_source with "Hv") as (sc_t [= ->]) "Hscrel".
+  iPoseProof (sc_rel_ptr_source with "Hscrel") as ([= ->]) "Htagged".
+  iApply (sim_retag_fnentry with "Hscrel Hcall"). 1: by cbv.
+  iIntros (t_i v_t v_s _ Hlen_t Hlen_s) "Hcall #Hvrel Htag_i Hi_t Hi_s".
+  destruct v_t as [|v_t []]; try done.
+  destruct v_s as [|v_s []]; try done. iSimpl in "Hcall".
   iApply sim_expr_base.
-  target_apply (Write _ _) (target_write_local with "Htag Ht") "Ht Htag"; [done | done | ].
-  source_apply (Write _ _) (source_write_local with "Htag Hs") "Hs Htag"; [done | done | ].
+  target_apply (Write _ _) (target_write_local with "Htag Ht") "Ht Htag".
+  2-3: done. 1: rewrite /write_range bool_decide_true. 2: simpl; lia. 1: rewrite Z.sub_diag /= //.
+  source_apply (Write _ _) (source_write_local with "Htag Hs") "Hs Htag".
+  2: done. 1: rewrite /write_range bool_decide_true. 2: simpl; lia. 1: rewrite Z.sub_diag /= //.
   sim_pures.
 
   (* do the source load *)
-  source_apply (Copy (Place _ _ _)) (source_copy_local with "Htag Hs") "Hs Htag"; first done.
+  source_apply (Copy (Place _ _ _)) (source_copy_local with "Htag Hs") "Hs Htag". 2: done.
+  1: rewrite read_range_heaplet_to_list // Z.sub_diag /= //.
   source_pures. source_bind (Copy _).
-  iApply (source_copy_any with "Htag_i Hi_s"); first done. iIntros (v_s' Hv_s') "Hi_s Htag_i". source_finish.
+  iApply (source_copy_protected with "Hcall Htag_i Hi_s"). 1,3: done. 3: rewrite lookup_insert //. 1: rewrite read_range_heaplet_to_list // Z.sub_diag /= //.
+  { intros off (?&?). simpl in *. assert (off = i.2) as -> by lia. rewrite /shift_loc /= Z.add_0_r lookup_insert. by eexists. }
+  iIntros "Hi_s Htag_i Hcall". source_finish.
   sim_pures.
 
   sim_apply (Call _ _) (Call _ _) (sim_call _ (ValR []) (ValR [])) ""; first by iApply value_rel_empty.
   iIntros (r_t r_s) "_". sim_pures.
 
   (* do the target load *)
-  target_apply (Copy (Place _ _ _)) (target_copy_local with "Htag Ht") "Ht Htag"; first done.
-  target_pures. target_apply (Copy _) (target_copy_protected with "Hcall Htag_i Hi_t") "Hi_t Hcall Htag_i"; first done.
-  { simpl. intros i0 Hi0. assert (i0 = O) as -> by lia. eexists. split; first apply lookup_insert.  set_solver. }
+  target_apply (Copy (Place _ _ _)) (target_copy_local with "Htag Ht") "Ht Htag". 2: done. 1: rewrite read_range_heaplet_to_list // Z.sub_diag /= //.
+  target_pures. target_apply (Copy _) (target_copy_protected with "Hcall Htag_i Hi_t") "Hi_t Htag_i Hcall". 1, 3: done. 3: rewrite lookup_insert //.
+  1: rewrite read_range_heaplet_to_list // Z.sub_diag /= //.
+  { intros off (?&?). simpl in *. assert (off = i.2) as -> by lia. rewrite /shift_loc /= Z.add_0_r lookup_insert. by eexists. }
   sim_pures.
 
   (* cleanup: remove the protector ghost state, make the external locations public, free the local locations*)
   sim_apply (Free _) (Free _) (sim_free_local with "Htag Ht Hs") "Htag"; [done..|]. sim_pures.
-  iApply (sim_protected_unprotectN with "Hcall Htag_i Hi_t Hi_s Hvrel"); [ | apply lookup_insert | ].
-  { simpl. cbn in Hlen_t. intros i' Hi'. replace i' with O by lia. rewrite elem_of_union elem_of_singleton. eauto. }
-  iIntros "Hcall Htag_i Hi_t Hi_s".
-  iApply (sim_remove_empty_calls t_i with "Hcall").
-  { rewrite lookup_insert. done. }
-  { rewrite Hlen_t. set_solver. }
-  iIntros "Hcall".
-  sim_apply (EndCall _) (EndCall _) (sim_endcall_own with "[Hcall]") "".
-  { replace (delete t_i _) with (∅ : gmap ptr_id (gset loc)); first done.
-    apply map_eq. intros t'. rewrite delete_insert_delete delete_insert; done.
-  }
+  iApply (sim_make_unique_public with "Hi_t Hi_s Htag_i Hcall Hvrel"). 1: by rewrite lookup_insert.
+  iIntros  "Htag_i Hcall". iEval (rewrite !fmap_insert !fmap_empty !insert_insert /=) in "Hcall".
+  iApply (sim_protected_unprotect_public with "Hcall Htag_i"). 1: by rewrite lookup_insert.
+  iIntros "Hc". iEval (rewrite delete_insert) in "Hc".
+  sim_apply (EndCall _) (EndCall _) (sim_endcall_own with "Hc") "".
   sim_pures.
-  sim_val. iModIntro. iSplit; first done.
-  destruct Hv_s' as [-> | ->]; first done.
-  iApply big_sepL2_forall. iSplit. { rewrite replicate_length. iPureIntro. lia. }
-  iIntros (k sc_t sc_s). rewrite lookup_replicate. iIntros "Hsc (-> & _)". destruct sc_t;done.
+  sim_val. iModIntro. iSplit; first done. done.
 Qed.
 
 Section closed.
