theories/tree_borrows/step_laws/steps_prot.v
@@ -82,7 +82,8 @@ Proof.
   - repeat (iSplit; first done).
     simpl. iIntros (l) "Hs". iPoseProof (state_rel_pub_or_priv with "Hs Hsrel") as "$".
   - (* call invariant *)
-    iPureIntro. intros c' M' HM'_some.
+    iPureIntro. destruct Hcall_interp as (Hcall_interp&Hcc2); split; last done.
+    intros c' M' HM'_some.
     specialize (Hcall_interp _ M' HM'_some) as (Hin & Hprot').
     split; first by apply Hin. intros pid L' HL_some. specialize (Hprot' _ _ HL_some) as [Hpid Hprot'].
     split; first by apply Hpid. intros l b Hin_l.
@@ -169,38 +170,6 @@ Proof.
 Qed.
 
 (*
-
-Lemma source_copy_protected v_s v_rd sz l_hl l_rd t π Ψ :
-  read_range l_rd.2 sz (list_to_heaplet v_s l_hl.2) = Some v_rd →
-  l_hl.1 = l_rd.1 →
-  t $$ tk_local -∗
-  l_hl ↦s∗[tk_local]{t} v_s -∗
-  (l_hl ↦s∗[tk_local]{t} v_s -∗ t $$ tk_local -∗ source_red #v_rd π Ψ)%E -∗
-  source_red (Copy (Place l_rd t sz)) π Ψ.
-Proof.
-  iIntros (Hread Hsameblk) "Htag Ht Hsim". eapply read_range_length in Hread as HH. subst sz.
-  iApply source_red_lift_base_step. iIntros (P_t σ_t P_s σ_s T_s K_s) "((HP_t & HP_s & Hbor)&%HT_s&%Hpool_safe)".
-  iPoseProof (bor_interp_get_state_wf with "Hbor") as "[%Hwf_t %]".
-  iModIntro. iDestruct "Hbor" as "(%M_call & %M_tag & %M_t & %M_s & Hbor)".
-  iPoseProof (bor_interp_readN_source_local with "Hbor Ht Htag") as "(%Hd & %it & %Hit & %Hitinv & %Hittag)".
-  opose proof* (read_range_list_to_heaplet_read_memory) as READ_MEM. 1: exact Hread. 1: done. 1: exact Hd.
-  destruct l_hl as [blk off_hl], l_rd as [blk2 off_rd]; simpl in *; subst blk2.
-  eapply mk_is_Some in Hread as Hrangebounds. rewrite -read_range_valid_iff in Hrangebounds.
-  setoid_rewrite <- list_to_heaplet_dom in Hrangebounds.
-  opose proof* (local_access_preserves_unchanged _ _ _ _ off_hl off_rd v_s (length v_rd)) as TREES_NOCHANGE. 3: exact Hd.
-  3: exists it; split; first done; split; first done; exact Hittag. 1: done.
-  { destruct v_rd as [|? v_rd]; first by left. simpl in *. right. split. 1: ospecialize (Hrangebounds off_rd _); try lia.
-    ospecialize (Hrangebounds (off_rd + (length v_rd)) _); lia. }
-  do 2 iExists _.
-  iSplit.
-  { iPureIntro. eapply copy_base_step'. 1: done. 2: exact READ_MEM. 2: exact TREES_NOCHANGE.
-    rewrite /trees_contain /trees_at_block /= Hit. subst t. cbv. tauto. }
-  iModIntro.
-  iSplitR "Htag Ht Hsim"; last first.
-  1: iApply ("Hsim" with "Ht Htag").
-  iFrame. destruct σ_s; simpl.
-  iExists _, _, _, _. iApply "Hbor".
-Qed.
 
 (** ** Write *)
 
